sub_find and sub_filter are now defined using ALFind, and ALFilter
did not delete lemmas about them to instead use the more
general lemmas about ALFind and
ALFilter, because that was taking too much time.

substitution.v
@@ -45,6 +45,7 @@ Require Import varInterface.
 Require Import terms.
 Require Import terms2.
 Require Import lmap.
+Require Import AssociationList.
 (** printing #  $\times$ #×# *)
 (** printing $  $\times$ #×# *)
 (** printing <=>  $\Leftrightarrow$ #&hArr;# *)
@@ -96,7 +97,7 @@ Notation oterm := (@oterm NVar Opid).
 Notation bterm := (@bterm NVar Opid).
 Notation vterm := (@vterm NVar Opid).
 
-Definition Substitution   : Type := lmap NVar NTerm.
+Definition Substitution   : Type := AssocList NVar NTerm.
 Definition WfSubstitution : Type := lmap NVar WTerm.
 Definition CSubstitution  : Type := lmap NVar  CTerm.
 
@@ -124,7 +125,7 @@ Definition dom_sub  (sub : Substitution) : list NVar := map (fun x => fst x) sub
 Definition Sub  := Substitution.
 Definition CSub := CSubstitution.
 
-Definition dom_sub : Substitution -> (list NVar):= @dom_lmap NVar NTerm.
+Definition dom_sub : Substitution -> (list NVar):= @ALDom NVar NTerm.
 Definition dom_csub   (sub : CSubstitution)  := map (fun x => fst x) sub.
 Definition wf_dom_sub (sub : WfSubstitution) := map (fun x => fst x) sub.
 
@@ -224,12 +225,9 @@ Proof using.
     apply Hsat in Hx;sp.
 Qed.
 
+Definition sub_find : forall (sub : Substitution) (var : NVar), option NTerm :=
+ @ALFind NVar NTerm _.
 
-Fixpoint sub_find (sub : Substitution) (var : NVar) : option NTerm :=
-  match sub with
-  | nil => None
-  | (v, t) :: xs => if beq_var v var then Some t else sub_find xs var
-  end.
 
 Lemma fold_var_ren :
   forall lvo lvn,
@@ -251,14 +249,11 @@ Definition  lmap_lapply {A : Type} (eqdec: Deq A) (sub: lmap A A)  (la:list A): 
 Definition  lvmap_lapply  (sub: lmap NVar NVar)  (la:list NVar): list NVar :=
   map (fun a:NVar =>  lmap_apply deq_nvar sub a) la.
 
-Definition proj_as_option {A Q: Type} {P : A->Type} (a': {a : A & (P a)} + Q)
-  : option A :=
-  match a' with
-    | inl (existT _ a' _) => Some a'
-    |  inr _ => None
-  end.
 
 Hint Rewrite deqP_refl.
+Hint Rewrite deq_refl.
+Hint Rewrite deqP_refl:SquiggleEq.
+Hint Rewrite deq_refl:SquiggleEq.
 Lemma sub_lmap_find: forall (sub: Substitution) v, sub_find sub v =
         proj_as_option (lmap_find deq_nvar sub v).
 Proof using.
@@ -383,15 +378,10 @@ Fixpoint lmap_filter {A B: Type}
   end.
 
 (* removes from sub the variables from vars *)
-Fixpoint sub_filter (sub : Substitution) (vars : list NVar) : Substitution :=
-  match sub with
-  | nil => nil
-  | (v, t) :: xs =>
-      if memvar v vars
-      then sub_filter xs vars
-      else (v, t) :: sub_filter xs vars
-  end.
 
+Definition sub_filter : 
+   forall (sub : Substitution) (vars : list NVar), Substitution :=
+ @ALFilter NVar NTerm _.
 
 
 Lemma sub_filter_subset :
@@ -556,7 +546,7 @@ Lemma dom_sub_app :
   forall sub1 sub2,
     dom_sub (sub1 ++ sub2) = dom_sub sub1 ++ dom_sub sub2.
 Proof using.
-  unfold dom_sub, dom_lmap; intros; rw map_app; auto.
+  unfold dom_sub, ALDom; intros; rw map_app; auto.
 Qed.
 
 
@@ -5177,7 +5167,7 @@ Hint Resolve disjoint_sym : slow.
 Lemma disjoint_dom_sub_filt : forall sub lv, 
   disjoint (dom_sub (sub_filter sub lv)) lv.
 Proof using. introv Hin Hinc.
-  unfold dom_sub, dom_lmap in Hin.
+  unfold dom_sub, ALDom in Hin.
   apply in_map_iff in Hin.
   exrepnd.
   allsimpl. subst.
@@ -5190,7 +5180,7 @@ Lemma disjoint_dom_sub_filt2 : forall sub lv1 lvn,
   -> disjoint (dom_sub (sub_filter sub lv1)) lvn.
 Proof using.
   introv Hdis Hin Hinc.
-  unfold dom_sub, dom_lmap in Hin.
+  unfold dom_sub, ALDom in Hin.
   apply in_map_iff in Hin.
   exrepnd.
   allsimpl. subst.
