UsefulTypes.v
@@ -585,6 +585,11 @@ Proof using.
   lia.
 Qed.
 
-
+Definition proj_as_option {A Q: Type} {P : A->Type} (a': {a : A & (P a)} + Q)
+   : option A :=
+   match a' with
+     | inl (existT _ a' _) => Some a'
+     |  inr _ => None
+   end.
 
 
